wip on ordered: asymmetric property proven but requires optimization

src/spec/Flutterbye.Seq.Ordered.fst
@@ -20,7 +20,7 @@ module Flutterbye.Seq.Ordered
 open FStar.Seq
 open Flutterbye.Seq.Mem
 
-type cmp_t 'a = 'a -> 'a -> Tot bool 
+type cmp_t 'a = 'a -> 'a -> Tot bool
 
 private type reflexive_p (#a_t:Type) (f:cmp_t a_t) (s:seq a_t)  =
    forall x.
@@ -28,33 +28,82 @@ private type reflexive_p (#a_t:Type) (f:cmp_t a_t) (s:seq a_t)  =
 
 private type antisymmetric_p (#a_t:Type) (f:cmp_t a_t) (s:seq a_t) =
    forall x y.
-      mem x s && mem y s && f x y && f y x <==> 
-         mem x s && mem y s && y = x  
+      mem x s && mem y s && f x y && f y x <==>
+         mem x s && mem y s && y = x
 
 private type transitive_p (#a_t:Type) (f:cmp_t a_t) (s:seq a_t) =
    forall x y z.
-      mem x s && mem y s && mem z s && f x y && f y z <==> 
-         mem x s && mem y s && mem z s && f x z  
+      mem x s && mem y s && mem z s && f x y && f y z <==>
+         mem x s && mem y s && mem z s && f x z
 
 type pordered_p (#a_t:Type) (f:cmp_t a_t) (s:seq a_t) =
    reflexive_p f s /\ antisymmetric_p f s /\ transitive_p f s
 
-private val antisymmetric_lemma: 
+private val reflexive_loop:
+   f:cmp_t 'a ->
+   s:seq 'a ->
+   i:nat{i <= length s /\ reflexive_p f (slice s 0 i)} ->
+   Tot (b:bool{b2t b <==> reflexive_p f s})
+      (decreases (length s - i))
+let rec reflexive_loop f s i =
+   if i < length s then
+      let a = index s i in
+      if f a a then
+         reflexive_loop f s (i + 1)
+      else
+         false
+   else
+      true
+
+private type antisymmetric_inner_p (#a_t:Type) (f:cmp_t a_t) (s:seq a_t) (a:a_t) =
+   forall x.
+      mem x s && f x a && f a x <==> mem x s && a = x
+
+private val antisymmetric_inner_loop:
+   f:cmp_t 'a ->
+   s:seq 'a ->
+   a:'a ->
+   i:nat{i <= length s /\ antisymmetric_inner_p f (slice s 0 i) a} ->
+   Tot (b:bool{b2t b <==> antisymmetric_inner_p f s a})
+      (decreases (length s - i))
+let rec antisymmetric_inner_loop f s a i =
+   if i < length s then
+      let a' = index s i in
+      if (a = a') = (f a a' && f a' a) then
+         antisymmetric_inner_loop f s a (i + 1)
+      else
+         false
+   else
+      true
+
+private val antisymmetric_loop:
+   f:cmp_t 'a ->
+   s:seq 'a ->
+   i:nat{i <= length s /\ antisymmetric_p f (slice s 0 i)} ->
+   Tot (b:bool{b2t b <==> antisymmetric_p f s})
+      (decreases (length s - i))
+let rec antisymmetric_loop f s i =
+   if i < length s then
+      let a = index s i in
+      if antisymmetric_inner_loop f s a 0 then
+         (assert (antisymmetric_p f (slice s 0 (i + 1))); // optimization
+         antisymmetric_loop f s (i + 1))
+      else
+         false
+   else
+      true
+
+(*
+
+
+private val antisymmetric_lemma:
    f:cmp_t 'a ->
    s:seq 'a ->
    a:'a ->
    Lemma
-      (ensures (antisymmetric_p f (append s (create 1 a))))
+      (ensures (pordered_p f (append s (create 1 a))))
 let antisymmetric_lemma f s a =
    admit ()
-
-private val still_antisymmetric:
-   f:cmp_t 'a ->
-   s:seq 'a{antisymmetric_p f s} ->
-   a:'a ->
-   Tot bool
-let still_antisymmetric f s a =
-
 
 private val pordered_loop:
    f:cmp_t 'a ->
@@ -65,7 +114,7 @@ private val pordered_loop:
 let rec pordered_loop f s i =
    if i < length s then
       let a = index s i in
-      if f a a then 
+      if f a a then //
          begin
             if i = 0 then
                pordered_loop f s 1
@@ -87,3 +136,4 @@ let rec pordered_loop f s i =
 val pordered: f:cmp_t 'a -> s:seq 'a -> Tot (b:bool{b <==> pordered_p f s})
 let pordered f s =
    pordered_loop f s 0
+*)
